reify/mirror_cancel.v
@@ -6,7 +6,9 @@ Require Import sep.
 Require Import FMapInterface.
 Require Import SimpleInstantiation.
 Require Import MirrorShard.ExprUnifySynGenRec.
-
+Require Import wrapExpr.
+Require Import Provers.
+Require Import reify_derives.
 
 Module SH := SepHeap.Make VericSepLogic Sep.
 Module SL := SepLemma VericSepLogic Sep.
@@ -17,4 +19,88 @@ Module UNF := Unfolder.Make VericSepLogic Sep SH SUBST UNIFY SL.
 
 Module CancelModule := CancelTacBedrock.Make VericSepLogic Sep SH SL SUBST UNIFY UNF.
 
-(*CancelModule.canceller some things...*)
+Definition reflect_e types functions meta_env var_env :=
+fun h => force_Opt (@Expr.exprD types functions meta_env var_env h Expr.tvProp) False.
+
+Lemma goalD_unfold :
+forall types funcs preds meta_env hyps l r,
+(Expr.AllProvable funcs meta_env nil hyps -> 
+derivesD types funcs preds meta_env nil (l, r)) -> goalD types funcs preds meta_env nil ((hyps, (l, r))). 
+intros. generalize dependent hyps.
+induction hyps; intros.
+unfold goalD. simpl. simpl in H.
+apply H. auto.
+simpl.
+intros.
+simpl in H.
+assert ((AllProvable funcs meta_env nil hyps ->
+            derivesD types funcs preds meta_env nil (l, r))).
+simpl. 
+intros.
+apply H. split.
+unfold Expr.Provable. destruct (Expr.exprD funcs meta_env nil a Expr.tvProp);
+auto.
+apply H1.
+intuition.
+simpl in *.
+destruct hyps. auto.
+assumption.
+Qed.
+
+
+Lemma ApplyCancelSep_with_eq_goal 
+(boundf boundb : nat) (types : list Expr.type) :
+      forall (meta_env : Expr.env types) (hyps : Expr.exprs types) preds funcs prover hintsFwd hintsBwd,
+      forall (l r : Sep.sexpr types) res,
+      forall (WTR : Sep.WellTyped_sexpr (Expr.typeof_funcs funcs) (Sep.typeof_preds preds) (Expr.typeof_env meta_env) nil r = true),
+       UNF.hintSideD funcs preds hintsFwd ->
+       UNF.hintSideD funcs preds hintsBwd ->
+       Prover.ProverT_correct prover funcs ->
+      CancelModule.canceller (Sep.typeof_preds preds) hintsFwd hintsBwd prover boundf boundb (Expr.typeof_env meta_env) hyps l r = Some res ->
+      match res with
+        | {| CancelModule.AllExt := new_vars
+           ; CancelModule.ExExt  := new_uvars
+           ; CancelModule.Lhs    := lhs'
+           ; CancelModule.Rhs    := rhs'
+           ; CancelModule.Subst  := subst
+          |} =>
+        Expr.forallEach new_vars (fun nvs : Expr.env types =>
+          let var_env := nvs in
+          Expr.AllProvable_impl funcs meta_env var_env
+          (CancelModule.INS.existsSubst funcs subst meta_env var_env (length meta_env) new_uvars
+            (fun meta_ext : Expr.env types =>
+              SUBST.Subst_equations_to funcs meta_ext var_env subst 0 meta_env /\
+              let meta_env := meta_ext in
+                (Expr.AllProvable_and funcs meta_env var_env
+                  (VericSepLogic.himp  
+                    (Sep.sexprD funcs preds meta_env var_env
+                      (SH.sheapD (SH.Build_SHeap (SH.impures lhs') nil (SH.other lhs'))))
+                    (Sep.sexprD funcs preds meta_env var_env
+                      (SH.sheapD (SH.Build_SHeap (SH.impures rhs') nil (SH.other rhs')))))
+                  (SH.pures rhs')) ))
+            (SH.pures lhs'))
+      end ->
+      goalD types funcs preds meta_env nil ((hyps, (l, r))).
+Proof.
+intros.
+apply goalD_unfold.
+intros.
+simpl.
+eapply CancelModule.ApplyCancelSep_with_eq.
+apply H.
+apply H0.
+apply X.
+apply Expr.typeof_funcs_WellTyped_funcs.
+reflexivity. 
+apply H3.
+auto.
+apply H1.
+auto.
+Qed.
+
+Ltac mirror_cancel boundf boundb prover prover_proof leftr rightr:=
+eapply (ApplyCancelSep_with_eq_goal boundf boundb _ _ _ _ _ prover leftr rightr); auto; try solve[ constructor]; try apply prover_proof.
+
+Ltac mirror_cancel_default :=
+let types := get_types in 
+eapply (ApplyCancelSep_with_eq_goal 100 100 _ _ _ _ _ (Provers.trivialProver types) nil nil); auto; try solve[ constructor]; try apply trivialProver_correct.
